\documentclass[12pt]{article}
\usepackage{amssymb}
\usepackage{amsmath}
\usepackage{amsthm}

\DeclareMathOperator{\arccot}{arccot}

\begin{document}


Thesis:

$$ \sum_{n=1}^{\infty} (-1)^n \ln \left(1 + \frac{1}{n} \right) = \ln \left( \frac{2}{\pi} \right) $$

Transforming:

\begin{eqnarray*}
\sum_{n=1}^{\infty} (-1)^n \ln \left(1 + \frac{1}{n} \right) &=& \displaystyle\sum_{n=1}^{\infty} (-1)^n \ln \left(\frac{n+1}{n} \right) \\
	&=& -\ln \left( \frac{2}{1}  \right) + \ln \left( \frac{3}{2}  \right) - \ln \left( \frac{4}{3}  \right) + \ln \left( \frac{5}{4}  \right) - \cdots \\
	&=& \ln \left( \frac{1}{2}  \right) + \ln \left( \frac{3}{2}  \right) + \ln \left( \frac{3}{4}  \right) + \ln \left( \frac{5}{4}  \right) + \cdots \\
	&=& \ln \left( \frac{1 \cdot 3}{2 \cdot 2}  \right) + \ln \left( \frac{3 \cdot 5}{4 \cdot 4}  \right) + \ln \left( \frac{5\cdot 7}{6\cdot 6}  \right) + \cdots \\
	&=& - \ln \left( \frac{2 \cdot 2}{1 \cdot 3} \cdot \frac{4 \cdot 4}{3 \cdot 5} \cdot \frac{5 \cdot 7}{6 \cdot 6} \cdot \cdots \right)
\end{eqnarray*}

Wallis product for $\pi$: 
$$ \frac{\pi}{2} = \frac{2 \cdot 2}{1 \cdot 3} \cdot \frac{4 \cdot 4}{3 \cdot 5} \cdot \frac{5 \cdot 7}{6 \cdot 6} \cdot \cdots $$

Hence:
$$ 
\sum_{n=1}^{\infty} (-1)^n \ln \left(1 + \frac{1}{n} \right) = - \ln \left( \frac{\pi}{2} \right) = \ln \left( \frac{2}{\pi} \right)
$$


\end{document}